# ğŸ“– æ•¸èˆ‡å¼

# â­• æ•¸èˆ‡å¼-å¼

## 1ï¸âƒ£ ä¹˜æ³•å…¬å¼

1. $$(a + b)^2 = a^2 + 2ab + b^2$$
2. $$(a - b)^2 = a^2 - 2ab + b^2$$
3. $$(a + b)^3 = a^3 + 3a^2b + 3ab^2 + b^3 \iff a^3 + b^3 = (a+b)^3 - 3ab(a+b)$$
4. $$(a - b)^3 = a^3 - 3a^2b + 3ab^2 - b^3 \iff a^3 - b^3 = (a-b)^3 + 3ab(a-b)$$
5. $$(a + b + c)^2 = a^2 + b^2 + c^2 + 2ab + 2bc + 2ac$$
6. $$(a_1 + a_2 + \dots + a_n)^2 = (a_1^2 + a_2^2 + \dots + a_n^2) + 2(a_1, a_2 \dots ä»»å…©æ•¸ä¹˜ç©)$$
   $$\rightarrow\[\left( \sum_{i=1}^{n} a_i \right)^2 = \sum_{i=1}^{n} a_i^2  + \sum_{1 \leq i < j \leq n} a_i a_j\]$$

---

**ğŸ“Œ ç¯„ä¾‹:**

> $$\text{ Q1: è‹¥ } a + b = 6, \quad ab = 3, \quad a > b, \quad \text{ æ±‚ } a - b = ? $$ $$ \text{ Q2: è¨­ } x^2 - 4x + 1 = 0, ~ \text{ å…©æ ¹ç‚º } \alpha, \beta, \text{ æ±‚ } \[ \alpha^2, \beta^2 \] \text{ åŠ } \[ \alpha^3, \beta^3 \] ? $$ $$ \text{ Q3: } t + \frac 1 t = 4, \text{ æ±‚ } \[ t^2 + \frac{1}{t^2} = ? \] \text{ åŠ } \[ t^3 + \frac{1}{t^3} = ? \] $$ ![Imgur](https://i.imgur.com/LILq1yM.jpg)

> $$
> Q: \text{æ±‚ } f(x) = (x+1)(x+2)(x+3)(x+4) \dots (x+10) \text{ çš„å±•é–‹å¼ï¼Ÿ} $$ $$ \rightarrow x^{10} \text{ çš„ä¿‚æ•¸ç‚º } 1$$ $$ \rightarrow x^9 \text{ çš„ä¿‚æ•¸ç‚º } \sum\_{k=1}^{10} k = \frac{10(1+10)}{2} = 55 $$ $$\rightarrow x^9 \text{ çš„ä¿‚æ•¸ç‚º} 1 \sim 10 \text{ ä»»å…©æ•¸å­—ä¹˜ç© }
> $$
>
> ![Imgur](https://imgur.com/SPS7tWZ.jpeg) ![Imgur](https://imgur.com/a8fxZq5.jpg)

**ğŸ’« è£œå……: æ±‚å’Œ (1.âˆ‘å…¬å¼, 2.åˆç‚ºå®šå€¼/å°æ¶ˆ)**

![Imgur](https://imgur.com/YHJQC1A.jpeg)

## 2ï¸âƒ£ åˆ†è§£å…¬å¼

7. $$a^2 - b^2 = (a + b)(a - b)$$
8. $$a^4 + a^2b^2 + b^4 = (a^2 + ab + b^2)(a^2 -ab + b^2)$$
9. $$a^3 + b^3 = (a + b)(a^2 - ab + b^2) = (a+b)^3 - 3ab(a+b)$$
10. $$a^3 - b^3 = (a - b)(a^2 + ab + b^2) = (a-b)^3 + 3ab(a-b)$$

```proof
8.  a^4 + (a^2)(b^2) + b^4 = (a^4 + 2(a^2)(b^2) + b^2) - (a^2)(b^2)
                          = [(a^2)(b^2)]^2 - (ab)^2
                          = (a^2 + ab + b^2)(a^2 - ab + b^2)

9.  a^3 + b^3 = (a+b)^3 -3(a^2)b - 3a(b^2) = (a+b)^3 - 3ab(a+b)
         = (a+b)[(a+b)^2 - 3ab] = (a+b)(a^2 + ab + b^2)

10. a^3 - b^3 = (a-b)^3 + 3(a^2)b - 3a(b^2) = (a-b)^3 - 3ab(a-b)
         = (a-b)[(a-b)^2 + 3ab] = (a-b)(a^2 + ab + b^2)
```

---

**ğŸ“Œ ç¯„ä¾‹:**

> $$\text{ åˆ†è§£ä¸‹åˆ—å„å¼å­: }$$
>
> $$
> \text{ Q1. }x^3 + 27 \text{ ? }
> $$
>
> $$
> \text{ Q2. }x^6 - 1 \text{ ? }
> $$
>
> $$
> \text{ Q3. }x^{12} + 7^6 \text{ ? }
> $$

```Sol
1. x^3 + 27 = (x - 3)(x^3 + 3x + 9)
2. (x^3 + 1)(x^3 - 1)
3. 3^{12} - 7^6 = (9^3 + 7^3)(9^3 - 7^3)
                = 16(81 - 63 + 49) x 2(81 + 63 + 49)
                = 17 x 67 x 2 x 193
```

```Proof
let 193 = a x b, a >= b > 1
        = a x b >= b^2 => (b <= 193^{1/2})
```

> $$\text{ Q1: è‹¥ 0 < x < 1, åŒ–ç°¡ } â€‹\sqrt{\smash[b]{x^2 + \frac{1}{x^2} + 2}} - â€‹\sqrt{\smash[b]{x^2 + \frac{1}{x^2} - 2}}$$
>
> $$\text{ Q2: è‹¥ b > a > 0, ä¸” } a^2 + b^2 = 6ab \text{ å‰‡ } \frac{a+b}{a-b} = ?$$
>
> $$\text{ Q3. è¨­ n ç‚ºæ­£æ•´æ•¸, ä¸” } n^4 - 23n^2 + 169 \text{ å”¯ä¸€è³ªæ•¸ } \text{ å‰‡æ­¤è³ªæ•¸ç‚ºä½•? }$$ ![Imgur](https://imgur.com/DYQaGfo.jpeg)

---
